Fix faulty replica model (#2573)
* Fix to take in consideration the Faulty replica's step.

* Simplified forall in InvNextFaulty.
Commented QuorumOfPreparesInNetworkMonotonic - currently
not part of the proof (it was used at an early stage of it
while debugging omissions in the replica model).

* Fixed QuorumOfPreparesInNetworkMonotonic lemma.

Fix to take in consideration both the Honest and Faulty
replicas' steps in reasoning about the Prepares in the network.

docs/sbft-formal-model/distributed_system.s.dfy
@@ -113,7 +113,7 @@ module DistributedSystem {
   predicate NextStep(c:Constants, v:Variables, v':Variables, step: Step) {
     && v.WF(c)
     && v'.WF(c)
-    && (ReplicaStep(c,v,v',step) || ClientStep(c,v,v',step))
+    && (ReplicaStep(c, v, v', step) || ClientStep(c, v, v', step) || FaultyReplicaStep(c, v, v', step))
     && (forall other | ValidHostId(other) && other != step.id :: v'.hosts[other] == v.hosts[other])
     && Network.Next(c.network, v.network, v'.network, step.msgOps, step.id)
   }
