docs/sbft-formal-model/proof.dfy
@@ -27,7 +27,7 @@ module Proof {
   import Replica
   import opened DistributedSystem
   import opened SafetySpec
-  import Library
+  import opened Library
 
   predicate IsHonestReplica(c:Constants, hostId:HostId) 
   {
@@ -434,13 +434,21 @@ module Proof {
     ProofCommitMsgsFromHonestSendersAgree(c, v, v', step);
   }
 
-  lemma QuorumOfPreparesInNetworkMonotonic(c: Constants, v:Variables, v':Variables, step:Step, h_step:Replica.Step)
+  lemma QuorumOfPreparesInNetworkMonotonic(c: Constants, v:Variables, v':Variables, step:Step)
     requires NextStep(c, v, v', step)
-    requires c.clusterConfig.IsReplica(step.id)
-    requires var h_c := c.hosts[step.id].replicaConstants;
-             var h_v := v.hosts[step.id].replicaVariables;
-             var h_v' := v'.hosts[step.id].replicaVariables;
-             Replica.NextStep(h_c, h_v, h_v', step.msgOps, h_step)
+    requires (c.clusterConfig.IsHonestReplica(step.id)
+              && var h_c := c.hosts[step.id].replicaConstants;
+                 var h_v := v.hosts[step.id].replicaVariables;
+                 var h_v' := v'.hosts[step.id].replicaVariables;
+                 var h_step :| Replica.NextStep(h_c, h_v, h_v', step.msgOps, h_step);
+                 Replica.NextStep(h_c, h_v, h_v', step.msgOps, h_step))
+              || 
+              (c.clusterConfig.IsFaultyReplica(step.id)
+               && var h_c := c.hosts[step.id].faultyReplicaConstants;
+                  var h_v := v.hosts[step.id].faultyReplicaVariables;
+                  var h_v' := v'.hosts[step.id].faultyReplicaVariables;
+                  var h_step :| FaultyReplica.NextStep(h_c, h_v, h_v', step.msgOps, h_step);
+                  FaultyReplica.NextStep(h_c, h_v, h_v', step.msgOps, h_step))
     ensures (forall view, seqID, clientOp | QuorumOfPreparesInNetwork(c, v, view, seqID, clientOp)
                                         :: QuorumOfPreparesInNetwork(c, v', view, seqID, clientOp))
   {
@@ -675,7 +683,7 @@ module Proof {
   {
     var step :| NextStep(c, v, v', step);
 
-    if (c.clusterConfig.IsReplica(step.id))
+    if (c.clusterConfig.IsHonestReplica(step.id))
     {
       var h_c := c.hosts[step.id].replicaConstants;
       var h_v := v.hosts[step.id].replicaVariables;
@@ -688,13 +696,13 @@ module Proof {
         case SendPrePrepareStep() => {
           SendPrePrepareStepPreservesInv(c, v, v', step, h_step);
         }
-        case RecvPrePrepareStep => {
+        case RecvPrePrepareStep() => {
           RecvPrePrepareStepPreservesInv(c, v, v', step, h_step);
         }
         case SendPrepareStep(seqID) => {
           SendPrepareStepPreservesInv(c, v, v', step, h_step);
         }
-        case RecvPrepareStep => { 
+        case RecvPrepareStep() => { 
           RecvPrepareStepPreservesInv(c, v, v', step, h_step);
         }
         case SendCommitStep(seqID) => {
@@ -717,10 +725,23 @@ module Proof {
         case SendClientOperationStep() => {
           SendClientOperationPreservesInv(c, v, v', step, h_step);
         }
-
+    } else if(c.clusterConfig.IsFaultyReplica(step.id)) {
+      InvNextFaulty(c, v, v', step);
+      CommitMsgStability(c, v, v', step);
     } else {
       assert false; // Should not be possible
     }
+  }
+
+  lemma InvNextFaulty(c: Constants, v:Variables, v':Variables, step: Step)
+    requires v.WF(c)
+    requires c.clusterConfig.IsFaultyReplica(step.id)
+    requires HonestReplicasLockOnCommitForGivenView(c, v)
+    requires NextStep(c, v, v', step)
+    ensures HonestReplicasLockOnCommitForGivenView(c, v')
+  {
+    reveal_HonestReplicasLockOnCommitForGivenView();
+    assert forall msg | msg in v'.network.sentMsgs && IsHonestReplica(c, msg.sender) :: msg in v.network.sentMsgs;
   }
 
   lemma InvariantInductive(c: Constants, v:Variables, v':Variables)
